\documentclass[11pt]{article}
%\setlength{\textwidth}{430pt}\setlength{\oddsidemargin}{11pt}
\usepackage{amssymb}
\usepackage{amsthm}
\usepackage{amsmath}
\usepackage{enumerate}
\usepackage{fancyhdr}
\usepackage[bottom=0.9in,top=0.9in]{geometry}
\usepackage{hyperref}
\hypersetup{colorlinks=true,linktoc=all,linkcolor=blue}

\begin{document}
\pagestyle{fancy}
\fancyhead{}
\fancyhead[C]{\textbf{Miscellaneous Exercises}}
\tableofcontents
\newpage
\section{Euclidean Geometry}
\subsection{Jane Street's 3b1b Puzzler}
Let $C$ be a closed bounded convex set in $\mathbb{R}^3$, and let $B = \partial C$.
Now imagine creating a new set by taking any two points from $B$ and adding them together, doing this for every possible pair of points.
Denote this new set of vector sums as $D = \{\vec{p}+\vec{q} \, | \,\vec{p},\vec{q} \in B\}$.\\
Prove that $D$ is also a convex set.
\begin{proof}
Let $\vec{x},\vec{y} \in D$. This implies that $\vec{x} = \vec{p} + \vec{q}$ and $\vec{y} = \vec{r} + \vec{s}$,
where $\vec{p},\vec{q},\vec{r},\vec{s} \in B$. It is first important to note that since $C$ is closed, it contains all its boundary points,
and since $C$ is bounded, the distance between any two boundary points is within the bound
defined by the distance function $d_C$, say $M \in \mathbb{R}$. Then, since $D$ is just the vector sums of all possible pairs of boundary points in $C$,
we can find the bound for $d_D$ with our given points in $D$ as follows:
\begin{equation*}
d_D(\vec{x},\vec{y}) = |\vec{x} - \vec{y}| = |(\vec{p} + \vec{q}) - (\vec{r} + \vec{s})| \leq |\vec{p} - \vec{r}| + |\vec{q} - \vec{s}| \leq M + M = 2M.
\end{equation*}
With this bound, let $\lambda \in \mathbb{R}$, where $0 < \lambda < 1$, and see that
\begin{align*}
|(1-\lambda)\vec{x} + \lambda\vec{y}| &= |\vec{x} - \lambda\vec{x} + \lambda\vec{y}| \\
                                      &= |(\vec{p}+\vec{q}) - \lambda(\vec{p}+\vec{q}) + \lambda(\vec{r} + \vec{s})| \\
                                      &= |\vec{p} - \lambda\vec{p} + \lambda\vec{r} + \vec{q} - \lambda\vec{q} + \lambda\vec{s}| \\
                                      &= |((1-\lambda)\vec{p} + \lambda\vec{r}) + ((1-\lambda)\vec{q} + \lambda\vec{s})| \\
                                      & \leq |(1-\lambda)\vec{p} + \lambda\vec{r}| + |(1-\lambda)\vec{q} + \lambda\vec{s})| \\
                                      & \leq M + M = 2M.
\end{align*}
Hence $(1-\lambda)\vec{x} + \lambda\vec{y} \in D$, implying that $D$ is indeed also a convex set.
\end{proof}

\newpage

\section{Calculus}
\subsection{The Math Sorcerers Calculus Problem His Students Couldn't Solve}
Find the equations of the tangent lines to the graph of $f(x) = x^2$ that pass through $(1,-1)$.
\renewcommand\qedsymbol{$\diagup\!\!\!\diagup$}
\begin{proof}[Solution]
Work in progress...
\end{proof}

\newpage

\section{Algebra}
\subsection{Exercise Posed During Lecture}
Simplify
\[\frac{1}{1+a+ab} + \frac{1}{1+b+bc} + \frac{1}{1+c+ca}\]
given that $abc=1$.
\begin{proof}[Solution]
Firstly, we will rearrange the first summand into
	\begin{equation*}
		\begin{aligned}
			\frac{1}{1+a+ab} &= \frac{1}{abc + a + ab} \\
			                 &= \frac{1}{a(bc + 1 + b)} \\
					 &= \frac{1}{a(1 + b + bc)} \\
					 &= \frac{1}{a(abc + b + bc)} \\
					 &= \frac{1}{ab(ac + 1 + c)} \\
					 &= \frac{1}{ab(1 + c + ca)}.
		\end{aligned}
	\end{equation*}
Then similarly, we will rearrange the second summand into
	\begin{equation*}
		\begin{aligned}
			\frac{1}{1+b+bc} &= \frac{1}{abc + b + bc} \\
			                 &= \frac{1}{b(ac + 1 + c)} \\
					 &= \frac{1}{b(1 + c + ca)}.
		\end{aligned}
	\end{equation*}
Now substitute both of these back into the original equation to get
	\begin{equation*}
		\begin{aligned}
			\frac{1}{1+a+ab} + \frac{1}{1+b+bc} + \frac{1}{1+c+ca} &= \frac{1}{ab(1 + c + ca)} + \frac{1}{b(1 + c + ca)} + \frac{1}{1+c+ca} \\
									       &= \frac{1}{1+c+ca}\left(\frac{1}{ab} + \frac{1}{b} + 1\right) \\
									       &= \frac{1}{1+c+ca}\left(\frac{1+a+ab}{ab}\right) \\
									       &= \frac{1+a+ab}{ab+abc+a^2bc} \\
									       &= \frac{1+a+ab}{ab+1+a} = 1.
		\end{aligned}
	\end{equation*}
\end{proof}
\renewcommand\qedsymbol{$square$}

\end{document}
